opentheory/examples/bits.ml
@@ -10,7 +10,7 @@ let bitwidth_def = new_definition
 export_thm bitwidth_def;;
 
 let num_bit_def = new_definition
-  `!n i. num_bit n i = ODD (n DIV (2 EXP n))`;;
+  `!n i. num_bit n i = ODD (n DIV (2 EXP i))`;;
 
 export_thm num_bit_def;;
 
@@ -19,224 +19,82 @@ let num_to_bits_def = new_definition
 
 export_thm num_to_bits_def;;
 
-let (bits_to_num_nil,num_to_bits_cons) =
+let is_bits_def = new_definition
+  `!l. is_bits l <=> NULL l \/ LAST l`;;
+
+export_thm is_bits_def;;
+
+let (bits_to_num_nil,bits_to_num_cons) =
   let def = new_recursive_definition list_RECURSION
     `(bits_to_num [] = 0) /\
      (!h t.
         bits_to_num (CONS h t) =
-        (if h then 1 else 0) + 2 * bits_to_num t)` in
+        2 * bits_to_num t + (if h then 1 else 0))` in
   CONJ_PAIR def;;
 
-export_thm bits_to_list_to_word_nil;;
-export_thm list_to_word_cons;;
+export_thm bits_to_num_nil;;
+export_thm bits_to_num_cons;;
 
-(*PARAMETRIC
-let list_to_word_nil = new_axiom
-  `list_to_word [] = num_to_word 0`
-and list_to_word_cons = new_axiom
-  `!h t.
-     list_to_word (CONS h t) =
-     if h then word_add (word_shl (list_to_word t) 1) (num_to_word 1)
-     else word_shl (list_to_word t) 1`;;
-*)
+let bits_to_num_def = CONJ bits_to_num_nil bits_to_num_cons;;
 
-let list_to_word_def = CONJ list_to_word_nil list_to_word_cons;;
+let rdecode_uniform_loop_exists = prove
+ (`!n w. ?loop. !r.
+     loop r =
+     let (l,r') = rbits w r in
+     let m = bits_to_num l in
+     if m < n then m else
+     loop r'`,
+  REPEAT GEN_TAC THEN
+  MP_TAC
+   (ISPECL
+      [`\ (r : random).
+          let (l,r') = rbits w r in
+          let m = bits_to_num l in
+          ~(m < n)`;
+       `\ (r : random).
+          let (l,r') = rbits w r in
+          let m = bits_to_num l in
+          r'`;
+       `\ (r : random).
+          let (l,r') = rbits w r in
+          let m = bits_to_num l in
+          m`] WF_REC_TAIL) THEN
+  DISCH_THEN
+    (X_CHOOSE_THEN `loop : random -> num`
+     STRIP_ASSUME_TAC) THEN
+  EXISTS_TAC `loop : random -> num` THEN
+  REPEAT GEN_TAC THEN
+  REWRITE_TAC [] THEN
+  FIRST_X_ASSUM (fun th -> CONV_TAC (LAND_CONV (ONCE_REWRITE_CONV [th]))) THEN
+  REWRITE_TAC [LET_DEF; LET_END_DEF] THEN
+  PAIR_CASES_TAC `rbits w r` THEN
+  DISCH_THEN
+    (X_CHOOSE_THEN `l : bool list`
+       (X_CHOOSE_THEN `r' : random` SUBST1_TAC)) THEN
+  REWRITE_TAC [] THEN
+  BOOL_CASES_TAC `bits_to_num l < n` THEN
+  REWRITE_TAC []);;
 
-(*PARAMETRIC
-let list_to_word_def = CONJ list_to_word_nil list_to_word_cons;;
-*)
+let rdecode_uniform_loop_def =
+  new_specification ["rdecode_uniform_loop"]
+    (ONCE_REWRITE_RULE [SKOLEM_THM]
+      (ONCE_REWRITE_RULE [SKOLEM_THM]
+        rdecode_uniform_loop_exists));;
 
-let is_word_list_def = new_definition
-  `!l. is_word_list (l : bool list) <=> LENGTH l = word_width`;;
+export_thm rdecode_uniform_loop_def;;
 
-(*PARAMETRIC
-new_constant ("is_word_list", `:bool list -> bool`);;
-*)
+let rdecode_uniform_def = new_definition
+  `!n r.
+     rdecode_uniform n r =
+     let w = bitwidth (n - 1) in
+     let (r1,r2) = rsplit r in
+     (rdecode_uniform_loop n w r1 MOD n, r2)`;;
 
-export_thm is_word_list_def;;
+export_thm rdecode_uniform_def;;
 
-(*PARAMETRIC
-let is_word_list_def = new_axiom
-  `!l. is_word_list (l : bool list) <=> LENGTH l = word_width`;;
-*)
-
-let word_and_def = new_definition
-  `!w1 w2.
-     word_and w1 w2 =
-     list_to_word (zipwith ( /\ ) (word_to_list w1) (word_to_list w2))`;;
-
-(*PARAMETRIC
-new_constant ("word_and", `:word -> word -> word`);;
-*)
-
-export_thm word_and_def;;
-
-(*PARAMETRIC
-let word_and_def = new_axiom
-  `!w1 w2.
-     word_and w1 w2 =
-     list_to_word (zipwith ( /\ ) (word_to_list w1) (word_to_list w2))`;;
-*)
-
-let word_or_def = new_definition
-  `!w1 w2.
-     word_or w1 w2 =
-     list_to_word (zipwith ( \/ ) (word_to_list w1) (word_to_list w2))`;;
-
-(*PARAMETRIC
-new_constant ("word_or", `:word -> word -> word`);;
-*)
-
-export_thm word_or_def;;
-
-(*PARAMETRIC
-let word_or_def = new_axiom
-  `!w1 w2.
-     word_or w1 w2 =
-     list_to_word (zipwith ( \/ ) (word_to_list w1) (word_to_list w2))`;;
-*)
-
-let word_not_def = new_definition
-  `!w. word_not w = list_to_word (MAP (~) (word_to_list w))`;;
-
-(*PARAMETRIC
-new_constant ("word_not", `:word -> word`);;
-*)
-
-export_thm word_not_def;;
-
-(*PARAMETRIC
-let word_not_def = new_axiom
-  `!w. word_not w = list_to_word (MAP (~) (word_to_list w))`;;
-*)
-
-let (word_bits_lte_nil,word_bits_lte_cons) =
-  let def = new_recursive_definition list_RECURSION
-    `(!q l. word_bits_lte q [] l = q) /\
-     (!q h t l.
-        word_bits_lte q (CONS h t) l =
-        word_bits_lte ((~h /\ HD l) \/ (~(h /\ ~HD l) /\ q)) t (TL l))` in
-  let wnil = prove
-    (`!q. word_bits_lte q [] [] = q`,
-     REWRITE_TAC [def])
-  and wcons = prove
-    (`!q h1 h2 t1 t2.
-        word_bits_lte q (CONS h1 t1) (CONS h2 t2) =
-        word_bits_lte ((~h1 /\ h2) \/ (~(h1 /\ ~h2) /\ q)) t1 t2`,
-     REWRITE_TAC [def; HD; TL]) in
-  (wnil,wcons);;
-
-(*PARAMETRIC
-new_constant ("word_bits_lte", `:bool -> bool list -> bool list -> bool`);;
-*)
-
-export_thm word_bits_lte_nil;;
-export_thm word_bits_lte_cons;;
-
-(*PARAMETRIC
-let word_bits_lte_nil = new_axiom
-   `!q. word_bits_lte q [] [] = q`
-and word_bits_lte_cons = new_axiom
-   `!q h1 h2 t1 t2.
-      word_bits_lte q (CONS h1 t1) (CONS h2 t2) =
-      word_bits_lte ((~h1 /\ h2) \/ (~(h1 /\ ~h2) /\ q)) t1 t2`;;
-*)
-
-let word_bits_lte_def = CONJ word_bits_lte_nil word_bits_lte_cons;;
-
-(*PARAMETRIC
-let word_bits_lte_def = CONJ word_bits_lte_nil word_bits_lte_cons;;
-*)
-
-logfile "word-bits-thm";;
-
-(*PARAMETRIC
-(* word-bits-thm *)
-*)
+logfile "natural-bits-thm";;
 
 (* Helper theorems (not exported) *)
-
-let even_zero = prove
-  (`!n. n = 0 ==> EVEN n`,
-   GEN_TAC THEN
-   DISCH_THEN SUBST_VAR_TAC THEN
-   REWRITE_TAC [EVEN]);;
-
-let cons_div_two = prove
-  (`!n h. (2 * n + (if h then 1 else 0)) DIV 2 = n`,
-   REPEAT GEN_TAC THEN
-   MATCH_MP_TAC EQ_TRANS THEN
-   EXISTS_TAC `(2 * n) DIV 2 + (if h then 1 else 0) DIV 2` THEN
-   CONJ_TAC THENL
-   [MP_TAC (SPECL [`2 * n`; `if h then 1 else 0`; `2`] DIV_ADD_MOD) THEN
-    COND_TAC THENL
-    [NUM_REDUCE_TAC;
-     ALL_TAC] THEN
-    DISCH_THEN (fun th -> REWRITE_TAC [GSYM th]) THEN
-    MP_TAC (SPECL [`2`; `n : num`] MOD_MULT) THEN
-    COND_TAC THENL
-    [NUM_REDUCE_TAC;
-     ALL_TAC] THEN
-    DISCH_THEN (fun th -> REWRITE_TAC [th; ADD]) THEN
-    BOOL_CASES_TAC `h:bool` THENL
-    [REWRITE_TAC [] THEN
-     NUM_REDUCE_TAC THEN
-     REWRITE_TAC [GSYM ODD_MOD; GSYM ADD1; ODD_DOUBLE];
-     REWRITE_TAC [] THEN
-     NUM_REDUCE_TAC THEN
-     REWRITE_TAC [GSYM EVEN_MOD; ADD_0; EVEN_DOUBLE]];
-    ALL_TAC] THEN
-   MP_TAC (SPECL [`2`; `n : num`] DIV_MULT) THEN
-   COND_TAC THENL
-   [NUM_REDUCE_TAC;
-    ALL_TAC] THEN
-   DISCH_THEN (fun th -> REWRITE_TAC [th; EQ_ADD_LCANCEL_0]) THEN
-   MATCH_MP_TAC DIV_LT THEN
-   BOOL_CASES_TAC `h : bool` THEN
-   REWRITE_TAC [] THEN
-   NUM_REDUCE_TAC);;
-
-let exp_two_nz = prove
-  (`!n. ~(2 EXP n = 0)`,
-   REWRITE_TAC [EXP_EQ_0] THEN
-   NUM_REDUCE_TAC);;
-
-let le_exp_two = prove
-  (`!m n. 2 EXP m <= 2 EXP n <=> m <= n`,
-   REWRITE_TAC [LE_EXP] THEN
-   NUM_REDUCE_TAC);;
-
-let lt_exp_two = prove
-  (`!m n. 2 EXP m < 2 EXP n <=> m < n`,
-   REWRITE_TAC [LT_EXP] THEN
-   NUM_REDUCE_TAC);;
-
-let lt_exp_two_suc = prove
-  (`!m n. m < 2 EXP n ==> 2 * m + 1 < 2 EXP SUC n`,
-   REPEAT STRIP_TAC THEN
-   MATCH_MP_TAC LTE_TRANS THEN
-   EXISTS_TAC `2 * (m + 1)` THEN
-   CONJ_TAC THENL
-   [REWRITE_TAC [LEFT_ADD_DISTRIB; LT_ADD_LCANCEL] THEN
-    NUM_REDUCE_TAC;
-    ALL_TAC] THEN
-   REWRITE_TAC [EXP; LE_MULT_LCANCEL] THEN
-   DISJ2_TAC THEN
-   ASM_REWRITE_TAC [GSYM ADD1; LE_SUC_LT]);;
-
-let mod_exp_two_lt = prove
-  (`!m n. m MOD (2 EXP n) < 2 EXP n`,
-   REPEAT GEN_TAC THEN
-   MP_TAC (SPECL [`m : num`; `2 EXP n`] DIVISION) THEN
-   COND_TAC THENL
-   [REWRITE_TAC [exp_two_nz];
-    DISCH_THEN (fun th -> ACCEPT_TAC (CONJUNCT2 th))]);;
-
-let div_exp_two_lt = prove
-  (`!m n. m DIV (2 EXP n) = 0 <=> m < 2 EXP n`,
-   REPEAT GEN_TAC THEN
-   MATCH_MP_TAC DIV_EQ_0 THEN
-   MATCH_ACCEPT_TAC exp_two_nz);;
 
 let cond_mod_two = prove
   (`!n. (if ODD n then 1 else 0) = n MOD 2`,
@@ -253,1211 +111,268 @@ let cond_mod_two = prove
     ASM_REWRITE_TAC [] THEN
     DISCH_THEN (fun th -> REWRITE_TAC [th])]);;
 
-let odd_mod_exp_two = prove
-  (`!m n. ODD (m MOD (2 EXP n)) <=> ODD m /\ ~(n = 0)`,
-   REPEAT GEN_TAC THEN
-   MP_TAC (SPEC `n:num` num_CASES) THEN
-   STRIP_TAC THENL
-   [ASM_REWRITE_TAC [EXP; MULT_CLAUSES; MOD_1; ODD];
-    ALL_TAC] THEN
-   POP_ASSUM SUBST_VAR_TAC THEN
-   REWRITE_TAC [NOT_SUC; EXP; ODD_MOD] THEN
-   AP_THM_TAC THEN
-   AP_TERM_TAC THEN
-   MATCH_MP_TAC MOD_MOD THEN
-   REWRITE_TAC [GSYM EXP; exp_two_nz]);;
-
-let mod_div_exp_two = prove
-  (`!x m n.
-      (x MOD (2 EXP m)) DIV (2 EXP n) =
-      (if m <= n then 0 else (x DIV (2 EXP n)) MOD (2 EXP (m - n)))`,
-   REPEAT GEN_TAC THEN
-   bool_cases_tac `m <= (n : num)` THENL
-   [ASM_REWRITE_TAC [] THEN
-    MATCH_MP_TAC DIV_LT THEN
-    MATCH_MP_TAC LTE_TRANS THEN
-    EXISTS_TAC `2 EXP m` THEN
-    ASM_REWRITE_TAC [le_exp_two; mod_exp_two_lt];
-    ALL_TAC] THEN
-   ASM_REWRITE_TAC [] THEN
-   MP_TAC (SPECL [`x : num`; `2 EXP n`; `2 EXP (m - n)`] DIV_MOD) THEN
-   COND_TAC THENL
-   [REWRITE_TAC [MULT_EQ_0; exp_two_nz];
-    ALL_TAC] THEN
-   DISCH_THEN (fun th -> REWRITE_TAC [th]) THEN
-   AP_THM_TAC THEN
-   AP_TERM_TAC THEN
-   AP_TERM_TAC THEN
-   REWRITE_TAC [GSYM EXP_ADD] THEN
-   AP_TERM_TAC THEN
-   MATCH_MP_TAC EQ_SYM THEN
-   MATCH_MP_TAC SUB_ADD2 THEN
-   MP_TAC (SPECL [`m:num`; `n:num`] LE_CASES) THEN
-   ASM_REWRITE_TAC []);;
-
 (* Exported theorems *)
 
-let length_word_to_list = prove
-  (`!w. LENGTH (word_to_list w) = word_width`,
-   REWRITE_TAC [word_to_list_def; LENGTH_MAP; length_interval]);;
+let length_num_to_bits = prove
+  (`!n. LENGTH (num_to_bits n) = bitwidth n`,
+   REWRITE_TAC [num_to_bits_def; LENGTH_MAP; length_interval]);;
 
-export_thm length_word_to_list;;
+export_thm length_num_to_bits;;
 
-(*PARAMETRIC
-let length_word_to_list = new_axiom
-  `!w. LENGTH (word_to_list w) = word_width`;;
-*)
+let bitwidth_zero = prove
+  (`bitwidth 0 = 0`,
+   REWRITE_TAC [bitwidth_def]);;
 
-let is_word_to_list = prove
-  (`!w. is_word_list (word_to_list w)`,
-   REWRITE_TAC [is_word_list_def; length_word_to_list]);;
+export_thm bitwidth_zero;;
 
-export_thm is_word_to_list;;
-
-(*PARAMETRIC
-let is_word_to_list = new_axiom
-  `!w. is_word_list (word_to_list w)`;;
-*)
-
-let word_bit_div = prove
-  (`!w n. word_bit w n = ODD (word_to_num w DIV (2 EXP n))`,
-   REWRITE_TAC [word_bit_def; word_shr_def; num_to_word_to_num] THEN
-   REPEAT GEN_TAC THEN
-   AP_TERM_TAC THEN
-   MATCH_MP_TAC mod_lt_word_size THEN
-   MATCH_MP_TAC LET_TRANS THEN
-   EXISTS_TAC `word_to_num w` THEN
-   CONJ_TAC THENL
-   [MATCH_MP_TAC DIV_LE THEN
-    REWRITE_TAC [EXP_EQ_0] THEN
-    NUM_REDUCE_TAC;
-    REWRITE_TAC [word_to_num_bound]]);;
-
-export_thm word_bit_div;;
-
-(*PARAMETRIC
-let word_bit_div = new_axiom
-  `!w n. word_bit w n = ODD (word_to_num w DIV (2 EXP n))`;;
-*)
-
-let nil_to_word_to_num = prove
-  (`word_to_num (list_to_word []) = 0`,
-   REWRITE_TAC [list_to_word_def; num_to_word_to_num] THEN
-   MATCH_MP_TAC mod_lt_word_size THEN
-   REWRITE_TAC [LT_NZ; word_size_nonzero]);;
-
-export_thm nil_to_word_to_num;;
-
-(*PARAMETRIC
-let nil_to_word_to_num = new_axiom
-  `word_to_num (list_to_word []) = 0`;;
-*)
-
-let cons_to_word_to_num = prove
-  (`!h t.
-      word_to_num (list_to_word (CONS h t)) =
-      (2 * word_to_num (list_to_word t) + (if h then 1 else 0)) MOD word_size`,
-   REWRITE_TAC [list_to_word_def] THEN
-   REPEAT STRIP_TAC THEN
-   MP_TAC (SPEC `h : bool` BOOL_CASES_AX) THEN
-   STRIP_TAC THENL
-   [ASM_REWRITE_TAC
-      [word_add_to_num; word_shl_def; EXP_1; word_to_num_to_word] THEN
-    REWRITE_TAC [num_to_word_to_num; mod_add_mod_word_size];
-    ASM_REWRITE_TAC [word_shl_def; EXP_1; word_to_num_to_word; ADD_0] THEN
-    REWRITE_TAC [num_to_word_to_num; mod_add_mod_word_size]]);;
-
-export_thm cons_to_word_to_num;;
-
-(*PARAMETRIC
-let cons_to_word_to_num = new_axiom
-   `!h t.
-      word_to_num (list_to_word (CONS h t)) =
-      (2 * word_to_num (list_to_word t) + (if h then 1 else 0)) MOD word_size`;;
-*)
-
-let list_to_word_to_num_bound = prove
-  (`!l. word_to_num (list_to_word l) < 2 EXP (LENGTH l)`,
-   LIST_INDUCT_TAC THENL
-   [REWRITE_TAC [nil_to_word_to_num; LENGTH; EXP] THEN
-    NUM_REDUCE_TAC;
-    ALL_TAC] THEN
-   REWRITE_TAC [cons_to_word_to_num; LENGTH] THEN
-   MATCH_MP_TAC LET_TRANS THEN
-   EXISTS_TAC `2 * word_to_num (list_to_word t) + (if h then 1 else 0)` THEN
-   CONJ_TAC THENL
-   [MATCH_MP_TAC MOD_LE THEN
-    ACCEPT_TAC word_size_nonzero;
-    ALL_TAC] THEN
-   MATCH_MP_TAC LET_TRANS THEN
-   EXISTS_TAC `2 * word_to_num (list_to_word t) + 1` THEN
-   CONJ_TAC THENL
-   [REWRITE_TAC [LE_ADD_LCANCEL] THEN
-    BOOL_CASES_TAC `h : bool`THEN
-    REWRITE_TAC [LE_REFL] THEN
-    NUM_REDUCE_TAC;
-    ALL_TAC] THEN
-   MATCH_MP_TAC lt_exp_two_suc THEN
-   FIRST_ASSUM ACCEPT_TAC);;
-
-export_thm list_to_word_to_num_bound;;
-
-(*PARAMETRIC
-let list_to_word_to_num_bound = new_axiom
-  `!l. word_to_num (list_to_word l) < 2 EXP (LENGTH l)`;;
-*)
-
-let list_to_word_to_num_bound_suc = prove
-  (`!l. 2 * word_to_num (list_to_word l) + 1 < 2 EXP (SUC (LENGTH l))`,
+let bitwidth_recursion = prove
+  (`!n. bitwidth n = if n = 0 then 0 else bitwidth (n DIV 2) + 1`,
    GEN_TAC THEN
-   MATCH_MP_TAC lt_exp_two_suc THEN
-   MATCH_ACCEPT_TAC list_to_word_to_num_bound);;
-
-export_thm list_to_word_to_num_bound_suc;;
-
-(*PARAMETRIC
-let list_to_word_to_num_bound_suc = new_axiom
-  `!l. 2 * word_to_num (list_to_word l) + 1 < 2 EXP (SUC (LENGTH l))`;;
-*)
-
-let cons_to_word_to_num_bound = prove
-  (`!h t.
-      2 * word_to_num (list_to_word t) + (if h then 1 else 0) <
-      2 EXP SUC (LENGTH t)`,
-   REPEAT GEN_TAC THEN
-   MATCH_MP_TAC LET_TRANS THEN
-   EXISTS_TAC `2 * word_to_num (list_to_word t) + 1` THEN
-   CONJ_TAC THENL
-   [REWRITE_TAC [LE_ADD_LCANCEL] THEN
-    BOOL_CASES_TAC `h : bool` THEN
-    REWRITE_TAC [LE_REFL; LE_0];
-    MATCH_ACCEPT_TAC list_to_word_to_num_bound_suc]);;
-
-export_thm cons_to_word_to_num_bound;;
-
-(*PARAMETRIC
-let cons_to_word_to_num_bound = new_axiom
-   `!h t.
-      2 * word_to_num (list_to_word t) + (if h then 1 else 0) <
-      2 EXP SUC (LENGTH t)`;;
-*)
-
-let word_to_list_to_word = prove
-  (`!w. list_to_word (word_to_list w) = w`,
-   GEN_TAC THEN
-   REWRITE_TAC [word_to_list_def] THEN
-   MATCH_MP_TAC word_to_num_inj THEN
-   MATCH_MP_TAC (ITAUT`!p q. (p ==> q) /\ p ==> q`) THEN
-   EXISTS_TAC
-     `!k.
-        k <= word_width ==>
-        word_to_num
-          (list_to_word (MAP (word_bit w) (interval (word_width - k) k))) =
-          word_to_num w DIV (2 EXP (word_width - k))` THEN
-   CONJ_TAC THENL
-   [DISCH_THEN (MP_TAC o SPEC `word_width`) THEN
-    REWRITE_TAC [SUB_REFL; LE_REFL; EXP; DIV_1];
-    ALL_TAC] THEN
-   MATCH_MP_TAC num_INDUCTION THEN
-   CONJ_TAC THENL
-   [REWRITE_TAC
-      [SUB_0; interval_def; MAP; nil_to_word_to_num; GSYM word_size_def;
-       word_to_num_div_bound];
-    ALL_TAC] THEN
-   REPEAT STRIP_TAC THEN
-   PAT_ASSUM `X ==> Y` THEN
-   COND_TAC THENL
-   [MATCH_MP_TAC LE_TRANS THEN
-    EXISTS_TAC `SUC k` THEN
-    ASM_REWRITE_TAC [LE; LE_REFL];
-    ALL_TAC] THEN
-   REWRITE_TAC [interval_def; MAP; cons_to_word_to_num] THEN
-   MP_TAC (SPECL [`word_width`; `k : num`] SUB_SUC_CANCEL) THEN
-   COND_TAC THENL
-   [ASM_REWRITE_TAC [GSYM LE_SUC_LT];
-    ALL_TAC] THEN
-   DISCH_THEN (SUBST1_TAC o SYM) THEN
-   DISCH_THEN SUBST1_TAC THEN
-   REWRITE_TAC [word_bit_div; cond_mod_two] THEN
-   ONCE_REWRITE_TAC [MULT_SYM] THEN
-   REWRITE_TAC [EXP] THEN
-   MP_TAC (SPECL [`word_to_num w`; `2 EXP (word_width - SUC k)`;
-                   `2`] (ONCE_REWRITE_RULE [MULT_SYM] DIV_DIV)) THEN
-   COND_TAC THENL
-   [REWRITE_TAC [GSYM EXP; EXP_EQ_0] THEN
-    NUM_REDUCE_TAC;
-    ALL_TAC] THEN
-   DISCH_THEN (fun th -> REWRITE_TAC [GSYM th]) THEN
-   MP_TAC (SPECL [`word_to_num w DIV (2 EXP (word_width - SUC k))`;
-                   `2`] DIVISION) THEN
-   COND_TAC THENL
-   [NUM_REDUCE_TAC;
-    ALL_TAC] THEN
-   DISCH_THEN (fun th -> REWRITE_TAC [GSYM (CONJUNCT1 th)]) THEN
-   MATCH_MP_TAC mod_lt_word_size THEN
-   MATCH_MP_TAC LET_TRANS THEN
-   EXISTS_TAC `word_to_num w` THEN
-   CONJ_TAC THENL
-   [MATCH_MP_TAC DIV_LE THEN
-    REWRITE_TAC [EXP_EQ_0] THEN
-    NUM_REDUCE_TAC;
-    REWRITE_TAC [word_to_num_bound]]);;
-
-export_thm word_to_list_to_word;;
-
-(*PARAMETRIC
-let word_to_list_to_word = new_axiom
-  `!w. list_to_word (word_to_list w) = w`;;
-*)
-
-let word_to_list_inj = prove
-  (`!w1 w2. word_to_list w1 = word_to_list w2 ==> w1 = w2`,
-   REPEAT STRIP_TAC THEN
-   ONCE_REWRITE_TAC [GSYM word_to_list_to_word] THEN
-   ASM_REWRITE_TAC []);;
-
-export_thm word_to_list_inj;;
-
-(*PARAMETRIC
-let word_to_list_inj = new_axiom
-  `!w1 w2. word_to_list w1 = word_to_list w2 ==> w1 = w2`;;
-*)
-
-let word_to_list_inj_eq = prove
-  (`!w1 w2. word_to_list w1 = word_to_list w2 <=> w1 = w2`,
-   REPEAT GEN_TAC THEN
-   EQ_TAC THENL
-   [MATCH_ACCEPT_TAC word_to_list_inj;
-    DISCH_THEN SUBST_VAR_TAC THEN
-    REFL_TAC]);;
-
-export_thm word_to_list_inj_eq;;
-
-(*PARAMETRIC
-let word_to_list_inj_eq = new_axiom
-  `!w1 w2. word_to_list w1 = word_to_list w2 <=> w1 = w2`;;
-*)
-
-let list_to_word_bit = prove
-  (`!l n.
-      word_bit (list_to_word l) n =
-      (n < word_width /\ n < LENGTH l /\ nth l n)`,
-   REWRITE_TAC [word_bit_div] THEN
-   ONCE_REWRITE_TAC [SWAP_FORALL_THM] THEN
-   INDUCT_TAC THENL
-   [LIST_INDUCT_TAC THENL
-    [REWRITE_TAC [LENGTH; nil_to_word_to_num; LT; ODD; EXP; DIV_1];
-     ALL_TAC] THEN
-    POP_ASSUM (K ALL_TAC) THEN
-    REWRITE_TAC
-      [LENGTH; cons_to_word_to_num; EXP; DIV_1; nth_zero; HD; LT_NZ; NOT_SUC] THEN
-    ASM_REWRITE_TAC [word_size_def; odd_mod_exp_two] THEN
-    CONV_TAC (RATOR_CONV (ONCE_REWRITE_CONV [CONJ_SYM])) THEN
-    AP_TERM_TAC THEN
-    BOOL_CASES_TAC `h:bool` THENL
-    [ASM_REWRITE_TAC [GSYM ADD1; ODD_DOUBLE];
-     ASM_REWRITE_TAC [ADD_0; GSYM NOT_EVEN; EVEN_DOUBLE]];
-    ALL_TAC] THEN
-   bool_cases_tac' `SUC n < word_width` THENL
-   [POP_ASSUM MP_TAC THEN
-    POP_ASSUM (K ALL_TAC) THEN
-    REPEAT STRIP_TAC THEN
-    ASM_REWRITE_TAC [NOT_ODD] THEN
-    MATCH_MP_TAC even_zero THEN
-    REWRITE_TAC [div_exp_two_lt] THEN
-    MATCH_MP_TAC LTE_TRANS THEN
-    EXISTS_TAC `word_size` THEN
-    REWRITE_TAC [word_to_num_bound] THEN
-    REWRITE_TAC [word_size_def; le_exp_two] THEN
-    ASM_REWRITE_TAC [GSYM NOT_LT];
-    ALL_TAC] THEN
-   ASM_REWRITE_TAC [] THEN
-   LIST_INDUCT_TAC THENL
-   [REWRITE_TAC [LENGTH; nil_to_word_to_num; LT; NOT_ODD] THEN
-    MATCH_MP_TAC even_zero THEN
-    REWRITE_TAC [div_exp_two_lt; LT_NZ; exp_two_nz];
-    ALL_TAC] THEN
-   POP_ASSUM (K ALL_TAC) THEN
-   REWRITE_TAC [LENGTH; cons_to_word_to_num; LT_SUC] THEN
-   MP_TAC (ISPECL [`h : bool`; `t : bool list`; `n : num`] nth_suc) THEN
-   MATCH_MP_TAC
-     (TAUT `!x y z w.
-              ((x /\ y <=> x /\ z) ==> w) ==>
-              ((x ==> (y <=> z)) ==> w)`) THEN
-   DISCH_THEN SUBST1_TAC THEN
-   REWRITE_TAC [word_size_def; mod_div_exp_two; GSYM NOT_LT] THEN
-   ASM_REWRITE_TAC [odd_mod_exp_two] THEN
-   SUBGOAL_THEN `~(word_width - SUC n = 0)` (fun th -> REWRITE_TAC [th]) THENL
-   [MP_TAC (SPECL [`word_width`; `SUC n`] SUB_EQ_0) THEN
-    COND_TAC THENL
-    [MATCH_MP_TAC LT_IMP_LE THEN
-     FIRST_ASSUM ACCEPT_TAC;
-     ALL_TAC] THEN
-    DISCH_THEN SUBST1_TAC THEN
-    STRIP_TAC THEN
-    UNDISCH_TAC `SUC n < word_width` THEN
-    ASM_REWRITE_TAC [NOT_LT; LE_REFL];
-    ALL_TAC] THEN
-   FIRST_X_ASSUM (fun th -> MP_TAC (SPEC `t : bool list` th)) THEN
-   KNOW_TAC `n < word_width` THENL
-   [MATCH_MP_TAC LT_TRANS THEN
-    EXISTS_TAC `SUC n` THEN
-    ASM_REWRITE_TAC [SUC_LT];
-    ALL_TAC] THEN
-   DISCH_THEN (fun th -> REWRITE_TAC [th]) THEN
-   DISCH_THEN (fun th -> REWRITE_TAC [GSYM th]) THEN
-   REWRITE_TAC [ODD_MOD] THEN
-   AP_THM_TAC THEN
-   AP_TERM_TAC THEN
-   AP_THM_TAC THEN
-   AP_TERM_TAC THEN
-   MATCH_MP_TAC EQ_TRANS THEN
-   EXISTS_TAC
-     `((2 * word_to_num (list_to_word t) + (if h then 1 else 0)) DIV 2) DIV
-      (2 EXP n)` THEN
-   CONJ_TAC THENL
-   [REWRITE_TAC [EXP] THEN
-    MATCH_MP_TAC EQ_SYM THEN
-    MATCH_MP_TAC DIV_DIV THEN
-    REWRITE_TAC [GSYM EXP; exp_two_nz];
-    ALL_TAC] THEN
-   AP_THM_TAC THEN
-   AP_TERM_TAC THEN
-   MATCH_ACCEPT_TAC cons_div_two);;
-
-export_thm list_to_word_bit;;
-
-(*PARAMETRIC
-let list_to_word_bit = new_axiom
-   `!l n.
-      word_bit (list_to_word l) n =
-      (n < word_width /\ n < LENGTH l /\ nth l n)`;;
-*)
-
-let short_list_to_word_to_list = prove
-  (`!l.
-      LENGTH l <= word_width ==>
-      word_to_list (list_to_word l) =
-      APPEND l (REPLICATE F (word_width - LENGTH l))`,
-   REWRITE_TAC [word_to_list_def; list_to_word_bit] THEN
-   REPEAT STRIP_TAC THEN
-   MATCH_MP_TAC nth_eq THEN
-   REWRITE_TAC [LENGTH_MAP; length_interval] THEN
-   CONJ_TAC THENL
-   [REWRITE_TAC [LENGTH_APPEND; LENGTH_REPLICATE] THEN
-    MATCH_MP_TAC EQ_SYM THEN
-    MATCH_MP_TAC SUB_ADD2 THEN
-    FIRST_ASSUM ACCEPT_TAC;
-    ALL_TAC] THEN
-   REPEAT STRIP_TAC THEN
-   MP_TAC (ISPECL [`word_bit (list_to_word l)`; `interval 0 word_width`;
-                   `i : num`] nth_map) THEN
-   COND_TAC THENL
-   [ASM_REWRITE_TAC [length_interval];
-    ALL_TAC] THEN
-   DISCH_THEN (fun th -> REWRITE_TAC [th]) THEN
-   MP_TAC (SPECL [`0`; `word_width`; `i : num`] nth_interval) THEN
-   ASM_REWRITE_TAC [ADD] THEN
-   DISCH_THEN (fun th -> REWRITE_TAC [th]) THEN
-   REWRITE_TAC [list_to_word_bit] THEN
-   MP_TAC (ISPECL [`l : bool list`;
-                   `REPLICATE F (word_width - LENGTH (l : bool list))`;
-                   `i : num`]
-                  nth_append) THEN
-   COND_TAC THENL
-   [REWRITE_TAC [LENGTH_REPLICATE] THEN
-    MATCH_MP_TAC LTE_TRANS THEN
-    EXISTS_TAC `word_width` THEN
-    ASM_REWRITE_TAC [] THEN
-    MP_TAC (SPEC `word_width` LE_REFL) THEN
-    MATCH_MP_TAC EQ_IMP THEN
-    AP_TERM_TAC THEN
-    MATCH_MP_TAC EQ_SYM THEN
-    MATCH_MP_TAC SUB_ADD2 THEN
-    FIRST_ASSUM ACCEPT_TAC;
-    ALL_TAC] THEN
-   DISCH_THEN SUBST1_TAC THEN
-   bool_cases_tac `i < LENGTH (l : bool list)` THENL
+   REWRITE_TAC [bitwidth_def] THEN
+   ASM_CASES_TAC `n = 0` THENL
    [ASM_REWRITE_TAC [];
-    ALL_TAC] THEN
-   ASM_REWRITE_TAC [] THEN
-   UNDISCH_TAC `i < word_width` THEN
-   POP_ASSUM MP_TAC THEN
-   POP_ASSUM (K ALL_TAC) THEN
-   REWRITE_TAC [NOT_LT; LE_EXISTS] THEN
-   DISCH_THEN (X_CHOOSE_THEN `d : num` SUBST_VAR_TAC) THEN
-   REWRITE_TAC [ADD_SUB2] THEN
-   STRIP_TAC THEN
-   MP_TAC (ISPECL [`F`;
-                   `word_width - LENGTH (l : bool list)`;
-                   `d : num`] nth_replicate) THEN
-   COND_TAC THENL
-   [MP_TAC (SPEC `LENGTH (l : bool list)` LT_ADD_LCANCEL) THEN
-    DISCH_THEN (fun th -> ONCE_REWRITE_TAC [GSYM th]) THEN
-    MATCH_MP_TAC LTE_TRANS THEN
-    EXISTS_TAC `word_width` THEN
-    ASM_REWRITE_TAC [] THEN
-    MP_TAC (SPEC `word_width` LE_REFL) THEN
-    MATCH_MP_TAC EQ_IMP THEN
-    AP_TERM_TAC THEN
-    MATCH_MP_TAC EQ_SYM THEN
-    ONCE_REWRITE_TAC [ADD_SYM] THEN
-    MATCH_MP_TAC SUB_ADD THEN
-    MATCH_MP_TAC LT_IMP_LE THEN
-    MATCH_MP_TAC LET_TRANS THEN
-    EXISTS_TAC `LENGTH (l : bool list) + d` THEN
-    ASM_REWRITE_TAC [LE_ADD];
-    DISCH_THEN (fun th -> REWRITE_TAC [th])]);;
+    ASM_REWRITE_TAC [EQ_ADD_RCANCEL] THEN
+    MP_TAC (SPECL [`2`; `n : num`] log_recursion) THEN
+    ANTS_TAC THENL
+    [ASM_REWRITE_TAC [TWO; SUC_LT];
+     DISCH_THEN SUBST1_TAC THEN
+     MP_TAC (SPECL [`n : num`; `2`] DIV_EQ_0) THEN
+     ANTS_TAC THENL
+     [ASM_REWRITE_TAC [TWO; NOT_SUC];
+      DISCH_THEN SUBST1_TAC THEN
+      REFL_TAC]]]);;
 
-export_thm short_list_to_word_to_list;;
+export_thm bitwidth_recursion;;
 
-(*PARAMETRIC
-let short_list_to_word_to_list = new_axiom
-   `!l.
-      LENGTH l <= word_width ==>
-      word_to_list (list_to_word l) =
-      APPEND l (REPLICATE F (word_width - LENGTH l))`;;
-*)
-
-let long_list_to_word_to_list = prove
-  (`!l.
-      word_width <= LENGTH l ==>
-      word_to_list (list_to_word l) = take word_width l`,
-   REWRITE_TAC [word_to_list_def; list_to_word_bit] THEN
-   REPEAT STRIP_TAC THEN
-   MATCH_MP_TAC nth_eq THEN
-   REWRITE_TAC [LENGTH_MAP; length_interval] THEN
-   CONJ_TAC THENL
-   [MATCH_MP_TAC EQ_SYM THEN
-    MATCH_MP_TAC length_take THEN
-    FIRST_ASSUM ACCEPT_TAC;
-    ALL_TAC] THEN
-   REPEAT STRIP_TAC THEN
-   MP_TAC (ISPECL [`word_bit (list_to_word l)`; `interval 0 word_width`;
-                   `i : num`] nth_map) THEN
-   COND_TAC THENL
-   [ASM_REWRITE_TAC [length_interval];
-    ALL_TAC] THEN
-   DISCH_THEN (fun th -> REWRITE_TAC [th]) THEN
-   MP_TAC (SPECL [`0`; `word_width`; `i : num`] nth_interval) THEN
-   ASM_REWRITE_TAC [ADD] THEN
-   DISCH_THEN (fun th -> REWRITE_TAC [th]) THEN
-   REWRITE_TAC [list_to_word_bit] THEN
-   ASM_REWRITE_TAC [] THEN
-   KNOW_TAC `i < LENGTH (l : bool list)` THENL
-   [MATCH_MP_TAC LTE_TRANS THEN
-    EXISTS_TAC `word_width` THEN
-    ASM_REWRITE_TAC [];
-    ALL_TAC] THEN
-   STRIP_TAC THEN
-   ASM_REWRITE_TAC [] THEN
-   MATCH_MP_TAC EQ_SYM THEN
-   MATCH_MP_TAC nth_take THEN
-   ASM_REWRITE_TAC []);;
-
-export_thm long_list_to_word_to_list;;
-
-(*PARAMETRIC
-let long_list_to_word_to_list = new_axiom
-   `!l.
-      word_width <= LENGTH l ==>
-      word_to_list (list_to_word l) = take word_width l`;;
-*)
-
-let list_to_word_to_list_eq = prove
-  (`!l.
-      word_to_list (list_to_word l) =
-      if LENGTH l <= word_width then
-        APPEND l (REPLICATE F (word_width - LENGTH l))
-      else
-        take word_width l`,
+let num_bit_zero = prove
+  (`!n. num_bit n 0 = ODD n`,
    GEN_TAC THEN
-   bool_cases_tac `LENGTH (l : bool list) <= word_width` THENL
-   [ASM_REWRITE_TAC [] THEN
-    MATCH_MP_TAC short_list_to_word_to_list THEN
-    FIRST_ASSUM ACCEPT_TAC;
+   REWRITE_TAC [num_bit_def; EXP_0; DIV_1]);;
+
+export_thm num_bit_zero;;
+
+let num_bit_suc = prove
+  (`!n i. num_bit n (SUC i) = num_bit (n DIV 2) i`,
+   REPEAT GEN_TAC THEN
+   REWRITE_TAC [num_bit_def; EXP] THEN
+   AP_TERM_TAC THEN
+   MATCH_MP_TAC EQ_SYM THEN
+   MATCH_MP_TAC DIV_DIV THEN
+   REWRITE_TAC [GSYM EXP_SUC; EXP_EQ_0; NOT_SUC; TWO]);;
+
+export_thm num_bit_suc;;
+
+let num_bit_div2 = prove
+  (`!n. num_bit (n DIV 2) = num_bit n o SUC`,
+   REWRITE_TAC [FUN_EQ_THM; num_bit_suc; o_THM]);;
+
+export_thm num_bit_div2;;
+
+let zero_num_bit = prove
+  (`!i. ~num_bit 0 i`,
+   GEN_TAC THEN
+   REWRITE_TAC [num_bit_def] THEN
+   MP_TAC (SPEC `2 EXP i` DIV_0) THEN
+   REWRITE_TAC [EXP_EQ_0] THEN
+   ANTS_TAC THENL
+   [REWRITE_TAC [TWO; NOT_SUC];
+    DISCH_THEN SUBST1_TAC THEN
+    REWRITE_TAC [ODD]]);;
+
+export_thm zero_num_bit;;
+
+let num_to_bits_recursion = prove
+  (`!n.
+      num_to_bits n =
+      if n = 0 then [] else CONS (ODD n) (num_to_bits (n DIV 2))`,
+   GEN_TAC THEN
+   REWRITE_TAC [num_to_bits_def] THEN
+   ASM_CASES_TAC `n = 0` THENL
+   [ASM_REWRITE_TAC [bitwidth_def; interval_zero; MAP];
     ASM_REWRITE_TAC [] THEN
-    MATCH_MP_TAC long_list_to_word_to_list THEN
-    MP_TAC (SPECL [`word_width`; `LENGTH (l : bool list)`] LE_CASES) THEN
-    ASM_REWRITE_TAC []]);;
+    CONV_TAC (LAND_CONV (ONCE_REWRITE_CONV [bitwidth_recursion])) THEN
+    ASM_REWRITE_TAC [interval_suc; GSYM ADD1; MAP] THEN
+    REWRITE_TAC [num_bit_zero; num_bit_div2; MAP_o; map_suc_interval]]);;
 
-export_thm list_to_word_to_list_eq;;
+export_thm num_to_bits_recursion;;
 
-(*PARAMETRIC
-let list_to_word_to_list_eq = new_axiom
-   `!l.
-      word_to_list (list_to_word l) =
-      if LENGTH l <= word_width then
-        APPEND l (REPLICATE F (word_width - LENGTH l))
-      else
-        take word_width l`;;
-*)
+let num_to_bits_eq_nil = prove
+  (`!n. num_to_bits n = [] <=> n = 0`,
+   GEN_TAC THEN
+   ONCE_REWRITE_TAC [num_to_bits_recursion] THEN
+   BOOL_CASES_TAC `n = 0` THEN
+   REWRITE_TAC [NOT_CONS_NIL]);;
 
-let list_to_word_to_list = prove
-  (`!l. LENGTH l = word_width <=> word_to_list (list_to_word l) = l`,
+export_thm num_to_bits_eq_nil;;
+
+let num_to_bits_zero = prove
+  (`num_to_bits 0 = []`,
+   REWRITE_TAC [num_to_bits_eq_nil]);;
+
+export_thm num_to_bits_zero;;
+
+let num_to_bits_one = prove
+  (`num_to_bits 1 = [T]`,
+   ONCE_REWRITE_TAC [num_to_bits_recursion] THEN
+   NUM_REDUCE_TAC THEN
+   REWRITE_TAC [num_to_bits_zero]);;
+
+export_thm num_to_bits_one;;
+
+let is_bits_nil = prove
+  (`is_bits []`,
+   REWRITE_TAC [is_bits_def; NULL]);;
+
+export_thm is_bits_nil;;
+
+let is_bits_num_to_bits = prove
+  (`!n. is_bits (num_to_bits n)`,
+   MATCH_MP_TAC div2_induction THEN
+   REPEAT STRIP_TAC THENL
+   [REWRITE_TAC [num_to_bits_zero; is_bits_nil];
+    ONCE_REWRITE_TAC [num_to_bits_recursion] THEN
+    ASM_REWRITE_TAC [] THEN
+    POP_ASSUM MP_TAC THEN
+    REWRITE_TAC [is_bits_def] THEN
+    (LIST_CASES_TAC `num_to_bits (n DIV 2)` THEN
+     STRIP_TAC THEN
+     ASM_REWRITE_TAC [NULL]) THENL
+    [POP_ASSUM MP_TAC THEN
+     REWRITE_TAC [num_to_bits_eq_nil] THEN
+     MP_TAC (SPECL [`n : num`; `2`] DIV_EQ_0) THEN
+     REWRITE_TAC [TWO; NOT_SUC] THEN
+     DISCH_THEN SUBST1_TAC THEN
+     ASM_REWRITE_TAC [LT; ONE] THEN
+     DISCH_THEN SUBST1_TAC THEN
+     REWRITE_TAC [ODD; LAST; NULL];
+     CONV_TAC (RAND_CONV (REWR_CONV LAST)) THEN
+     REWRITE_TAC [NULL]]]);;
+
+export_thm is_bits_num_to_bits;;
+
+let num_to_bits_to_num = prove
+  (`!n. bits_to_num (num_to_bits n) = n`,
+   MATCH_MP_TAC div2_induction THEN
+   REPEAT STRIP_TAC THENL
+   [REWRITE_TAC [num_to_bits_zero; bits_to_num_def];
+    ONCE_REWRITE_TAC [num_to_bits_recursion] THEN
+    ASM_REWRITE_TAC [bits_to_num_def; cond_mod_two] THEN
+    ONCE_REWRITE_TAC [MULT_SYM] THEN
+    MATCH_MP_TAC DIVISION_DEF_DIV THEN
+    REWRITE_TAC [TWO; NOT_SUC]]);;
+
+export_thm num_to_bits_to_num;;
+
+let bits_to_num_cons_div2 = prove
+  (`!h t. bits_to_num (CONS h t) DIV 2 = bits_to_num t`,
+   REPEAT GEN_TAC THEN
+   REWRITE_TAC [bits_to_num_def] THEN
+   ONCE_REWRITE_TAC [MULT_SYM] THEN
+   MP_TAC
+     (SPECL [`bits_to_num t`; `if h then 1 else 0`; `2`]
+        DIV_MULT_ADD) THEN
+   ANTS_TAC THENL
+   [REWRITE_TAC [TWO; NOT_SUC];
+    DISCH_THEN SUBST1_TAC THEN
+    REWRITE_TAC [EQ_ADD_LCANCEL_0] THEN
+    BOOL_CASES_TAC `h : bool` THEN
+    NUM_REDUCE_TAC]);;
+
+export_thm bits_to_num_cons_div2;;
+
+let num_bit_bits_to_num = prove
+  (`!l i. num_bit (bits_to_num l) i <=> i < LENGTH l /\ nth l i`,
+   LIST_INDUCT_TAC THENL
+   [REWRITE_TAC [bits_to_num_def; zero_num_bit; LENGTH; LT];
+    GEN_TAC THEN
+    NUM_CASES_TAC `i : num` THENL
+    [DISCH_THEN SUBST1_TAC THEN
+     REWRITE_TAC [LENGTH; LT_0; nth_zero; num_bit_zero] THEN
+     REWRITE_TAC [bits_to_num_def; ODD_ADD] THEN
+     SUBGOAL_THEN `ODD (2 * bits_to_num t) <=> F` SUBST1_TAC THENL
+     [REWRITE_TAC [NOT_ODD; EVEN_DOUBLE];
+      REWRITE_TAC [] THEN
+      BOOL_CASES_TAC `h : bool` THEN
+      REWRITE_TAC [ONE; ODD]];
+     STRIP_TAC THEN
+     ASM_REWRITE_TAC [num_bit_suc; LENGTH; LT_SUC; bits_to_num_cons_div2] THEN
+     POP_ASSUM_LIST (K ALL_TAC) THEN
+     ASM_CASES_TAC `n < LENGTH (t : bool list)` THENL
+     [ASM_REWRITE_TAC [] THEN
+      MATCH_MP_TAC EQ_SYM THEN
+      MATCH_MP_TAC nth_suc THEN
+      FIRST_ASSUM ACCEPT_TAC;
+      ASM_REWRITE_TAC []]]]);;
+
+export_thm num_bit_bits_to_num;;
+
+let is_bits_bitwidth = prove
+  (`!l. is_bits l <=> bitwidth (bits_to_num l) = LENGTH l`,
+   LIST_INDUCT_TAC THENL
+   [REWRITE_TAC [is_bits_nil; bits_to_num_nil; bitwidth_zero; LENGTH];
+    ONCE_REWRITE_TAC [bitwidth_recursion] THEN
+    REWRITE_TAC [LENGTH; bits_to_num_cons_div2; GSYM ADD1] THEN
+    ASM_CASES_TAC `bits_to_num (CONS h t) = 0` THENL
+    [ASM_REWRITE_TAC [NOT_SUC; is_bits_def; NULL] THEN
+     POP_ASSUM MP_TAC THEN
+     POP_ASSUM (K ALL_TAC) THEN
+     SPEC_TAC (`h : bool`, `b : bool`) THEN
+     SPEC_TAC (`t : bool list`, `l : bool list`) THEN
+     LIST_INDUCT_TAC THENL
+     [GEN_TAC THEN
+      REWRITE_TAC [LAST; NULL; bits_to_num_def; ADD_EQ_0; MULT_0] THEN
+      BOOL_CASES_TAC `b : bool` THEN
+      REWRITE_TAC [ONE; NOT_SUC];
+      GEN_TAC THEN
+      ONCE_REWRITE_TAC [bits_to_num_def] THEN
+      REWRITE_TAC [LAST_MULTIPLE; NULL; ADD_EQ_0; MULT_EQ_0] THEN
+      NUM_REDUCE_TAC THEN
+      STRIP_TAC THEN
+      FIRST_X_ASSUM MATCH_MP_TAC THEN
+      FIRST_ASSUM ACCEPT_TAC];
+     ASM_REWRITE_TAC [SUC_INJ] THEN
+     POP_ASSUM MP_TAC THEN
+     POP_ASSUM MP_TAC THEN
+     REWRITE_TAC [is_bits_def; NULL; LAST] THEN
+     LIST_CASES_TAC `t : bool list` THENL
+     [DISCH_THEN SUBST_VAR_TAC THEN
+      REWRITE_TAC
+        [NULL; LENGTH; bits_to_num_def; bitwidth_zero; MULT_0; ZERO_ADD] THEN
+      BOOL_CASES_TAC `h : bool` THEN
+      REWRITE_TAC [ONE; NOT_SUC];
+      DISCH_THEN
+        (X_CHOOSE_THEN `b : bool`
+          (X_CHOOSE_THEN `l : bool list` SUBST_VAR_TAC)) THEN
+      REWRITE_TAC [NULL] THEN
+      DISCH_THEN SUBST1_TAC THEN
+      REWRITE_TAC []]]]);;
+
+export_thm is_bits_bitwidth;;
+
+let bits_to_num_to_bits = prove
+  (`!l. is_bits l <=> num_to_bits (bits_to_num l) = l`,
    GEN_TAC THEN
    EQ_TAC THENL
-   [STRIP_TAC THEN
-    MATCH_MP_TAC EQ_TRANS THEN
-    EXISTS_TAC `take (LENGTH (l : bool list)) l` THEN
-    CONJ_TAC THENL
-    [ASM_REWRITE_TAC [] THEN
-     MATCH_MP_TAC long_list_to_word_to_list THEN
-     ASM_REWRITE_TAC [LE_REFL];
-     MATCH_ACCEPT_TAC take_length];
-    DISCH_THEN (fun th -> ONCE_REWRITE_TAC [GSYM th]) THEN
-    MATCH_ACCEPT_TAC length_word_to_list]);;
-
-export_thm list_to_word_to_list;;
-
-(*PARAMETRIC
-let list_to_word_to_list = new_axiom
-  `!l. LENGTH l = word_width <=> word_to_list (list_to_word l) = l`;;
-*)
-
-let word_shl_list = prove
-  (`!l n.
-      word_shl (list_to_word l) n =
-      list_to_word (APPEND (REPLICATE F n) l)`,
-   REWRITE_TAC [word_shl_def] THEN
-   REPEAT GEN_TAC THEN
-   MATCH_MP_TAC word_to_num_inj THEN
-   REWRITE_TAC [num_to_word_to_num] THEN
-   SPEC_TAC (`n:num`,`n:num`) THEN
-   MATCH_MP_TAC num_INDUCTION THEN
-   CONJ_TAC THENL
-   [REWRITE_TAC [EXP; REPLICATE; APPEND; MULT_CLAUSES] THEN
-    REWRITE_TAC [GSYM num_to_word_to_num; word_to_num_to_word];
-    ALL_TAC] THEN
-   REPEAT STRIP_TAC THEN
-   REWRITE_TAC [REPLICATE; APPEND; cons_to_word_to_num; ADD_0] THEN
-   POP_ASSUM (fun th -> REWRITE_TAC [GSYM th]) THEN
-   MP_TAC (SPECL [`2`; `word_size`; `2 EXP n * word_to_num (list_to_word l)`]
-                 MOD_MULT_RMOD) THEN
-   COND_TAC THENL
-   [ACCEPT_TAC word_size_nonzero;
-    ALL_TAC] THEN
-   DISCH_THEN (fun th -> REWRITE_TAC [th]) THEN
-   REWRITE_TAC [EXP; MULT_ASSOC]);;
-
-export_thm word_shl_list;;
-
-(*PARAMETRIC
-let word_shl_list = new_axiom
-   `!l n.
-      word_shl (list_to_word l) n =
-      list_to_word (APPEND (REPLICATE F n) l)`;;
-*)
-
-let short_word_shr_list = prove
-  (`!l n.
-      LENGTH l <= word_width ==>
-      word_shr (list_to_word l) n =
-      (if LENGTH l <= n then list_to_word []
-       else list_to_word (drop n l))`,
-   REWRITE_TAC [word_shr_def] THEN
-   REPEAT STRIP_TAC THEN
-   MATCH_MP_TAC word_to_num_inj THEN
-   REWRITE_TAC [num_to_word_to_num] THEN
-   bool_cases_tac `LENGTH (l : bool list) <= n` THENL
-   [ASM_REWRITE_TAC [] THEN
-    REWRITE_TAC [nil_to_word_to_num] THEN
-    MP_TAC (SPEC `word_size` MOD_0) THEN
-    COND_TAC THENL
-    [ACCEPT_TAC word_size_nonzero;
-     ALL_TAC] THEN
-    DISCH_THEN (fun th -> ONCE_REWRITE_TAC [GSYM th]) THEN
-    AP_THM_TAC THEN
-    AP_TERM_TAC THEN
-    MATCH_MP_TAC DIV_LT THEN
-    MATCH_MP_TAC LTE_TRANS THEN
-    EXISTS_TAC `2 EXP LENGTH (l : bool list)` THEN
-    CONJ_TAC THENL
-    [MATCH_ACCEPT_TAC list_to_word_to_num_bound;
-     ALL_TAC] THEN
-    ASM_REWRITE_TAC [LE_EXP] THEN
-    NUM_REDUCE_TAC;
-    ALL_TAC] THEN
-   ASM_REWRITE_TAC [] THEN
-   KNOW_TAC `n <= LENGTH (l : bool list)` THENL
-   [MATCH_MP_TAC LT_IMP_LE THEN
-    ASM_REWRITE_TAC [GSYM NOT_LE];
-    ALL_TAC] THEN
-   POP_ASSUM (K ALL_TAC) THEN
-   POP_ASSUM MP_TAC THEN
-   SPEC_TAC (`n:num`,`n:num`) THEN
-   SPEC_TAC (`l : bool list`,`l : bool list`) THEN
-   LIST_INDUCT_TAC THENL
-   [REWRITE_TAC [LE; LENGTH] THEN
+   [REWRITE_TAC [is_bits_bitwidth] THEN
+    STRIP_TAC THEN
+    MATCH_MP_TAC nth_eq THEN
+    ASM_REWRITE_TAC [length_num_to_bits] THEN
     REPEAT STRIP_TAC THEN
-    ASM_REWRITE_TAC [nil_to_word_to_num; drop_zero] THEN
-    NUM_REDUCE_TAC THEN
-    MATCH_MP_TAC MOD_0 THEN
-    ACCEPT_TAC word_size_nonzero;
-    ALL_TAC] THEN
-   GEN_TAC THEN
-   MP_TAC (SPEC `n : num` num_CASES) THEN
-   STRIP_TAC THENL
-   [DISCH_THEN (K ALL_TAC) THEN
-    DISCH_THEN (K ALL_TAC) THEN
-    ASM_REWRITE_TAC [EXP; DIV_1; drop_zero] THEN
-    MATCH_MP_TAC MOD_LT THEN
-    MATCH_ACCEPT_TAC word_to_num_bound;
-    ALL_TAC] THEN
-   POP_ASSUM SUBST_VAR_TAC THEN
-   REWRITE_TAC [LENGTH; LE_SUC; cons_to_word_to_num] THEN
-   REPEAT STRIP_TAC THEN
-   MP_TAC (ISPECL [`n' : num`; `h : bool`; `t : bool list`] drop_suc) THEN
-   ASM_REWRITE_TAC [] THEN
-   DISCH_THEN SUBST1_TAC THEN
-   FIRST_X_ASSUM (fun th -> MP_TAC (SPEC `n' : num` th)) THEN
-   COND_TAC THENL
-   [MATCH_MP_TAC LE_TRANS THEN
-    EXISTS_TAC `SUC (LENGTH (t : bool list))` THEN
-    ASM_REWRITE_TAC [SUC_LE];
-    ALL_TAC] THEN
-   COND_TAC THENL
-   [FIRST_ASSUM ACCEPT_TAC;
-    ALL_TAC] THEN
-   DISCH_THEN (fun th -> REWRITE_TAC [GSYM th]) THEN
-   AP_THM_TAC THEN
-   AP_TERM_TAC THEN
-   MATCH_MP_TAC EQ_TRANS THEN
-   EXISTS_TAC
-     `(2 * word_to_num (list_to_word t) + (if h then 1 else 0)) DIV
-      (2 EXP SUC n')` THEN
-   CONJ_TAC THENL
-   [AP_THM_TAC THEN
-    AP_TERM_TAC THEN
-    MATCH_MP_TAC MOD_LT THEN
-    MATCH_MP_TAC LTE_TRANS THEN
-    EXISTS_TAC `2 EXP SUC (LENGTH (t : bool list))` THEN
-    CONJ_TAC THENL
-    [MATCH_ACCEPT_TAC cons_to_word_to_num_bound;
-     ALL_TAC] THEN
-    ASM_REWRITE_TAC [word_size_def; le_exp_two];
-    ALL_TAC] THEN
-   MATCH_MP_TAC EQ_TRANS THEN
-   EXISTS_TAC
-     `((2 * word_to_num (list_to_word t) + (if h then 1 else 0)) DIV 2) DIV
-      (2 EXP n')` THEN
-   CONJ_TAC THENL
-   [REWRITE_TAC [EXP] THEN
-    MATCH_MP_TAC EQ_SYM THEN
-    MATCH_MP_TAC DIV_DIV THEN
-    REWRITE_TAC [GSYM EXP; exp_two_nz];
-    ALL_TAC] THEN
-   AP_THM_TAC THEN
-   AP_TERM_TAC THEN
-   MATCH_ACCEPT_TAC cons_div_two);;
+    ASM_REWRITE_TAC [num_to_bits_def] THEN
+    MP_TAC (ISPECL [`num_bit (bits_to_num l)`;
+                    `interval 0 (LENGTH (l : bool list))`;
+                    `i : num`] nth_map) THEN
+    ASM_REWRITE_TAC [length_interval] THEN
+    DISCH_THEN SUBST1_TAC THEN
+    MP_TAC (SPECL [`0`; `LENGTH (l : bool list)`; `i : num`] nth_interval) THEN
+    ASM_REWRITE_TAC [ZERO_ADD] THEN
+    DISCH_THEN SUBST1_TAC THEN
+    ASM_REWRITE_TAC [num_bit_bits_to_num];
+    STRIP_TAC THEN
+    ASM_REWRITE_TAC [is_bits_bitwidth] THEN
+    POP_ASSUM (CONV_TAC o RAND_CONV o RAND_CONV o REWR_CONV o SYM) THEN
+    REWRITE_TAC [length_num_to_bits]]);;
 
-export_thm short_word_shr_list;;
-
-(*PARAMETRIC
-let short_word_shr_list = new_axiom
-   `!l n.
-      LENGTH l <= word_width ==>
-      word_shr (list_to_word l) n =
-      (if LENGTH l <= n then list_to_word []
-       else list_to_word (drop n l))`;;
-*)
-
-let long_word_shr_list = prove
-  (`!l n.
-      word_width <= LENGTH l ==>
-      word_shr (list_to_word l) n =
-      if word_width <= n then list_to_word []
-      else list_to_word (drop n (take word_width l))`,
-   REPEAT STRIP_TAC THEN
-   MP_TAC (SPEC `l : bool list` long_list_to_word_to_list) THEN
-   COND_TAC THENL
-   [FIRST_ASSUM ACCEPT_TAC;
-    ALL_TAC] THEN
-   DISCH_THEN (fun th -> REWRITE_TAC [GSYM th]) THEN
-   CONV_TAC
-     (LAND_CONV
-        (LAND_CONV (ONCE_REWRITE_CONV [GSYM word_to_list_to_word]))) THEN
-   MP_TAC (SPEC `list_to_word l` length_word_to_list) THEN
-   DISCH_THEN (fun th -> REWRITE_TAC [GSYM th] THEN ASSUME_TAC th) THEN
-   MATCH_MP_TAC short_word_shr_list THEN
-   ASM_REWRITE_TAC [LE_REFL]);;
-
-export_thm long_word_shr_list;;
-
-(*PARAMETRIC
-let long_word_shr_list = new_axiom
-   `!l n.
-      word_width <= LENGTH l ==>
-      word_shr (list_to_word l) n =
-      if word_width <= n then list_to_word []
-      else list_to_word (drop n (take word_width l))`;;
-*)
-
-let word_shr_list = prove
-  (`!l n.
-      word_shr (list_to_word l) n =
-      (if LENGTH l <= word_width then
-         if LENGTH l <= n then list_to_word []
-         else list_to_word (drop n l)
-       else
-         if word_width <= n then list_to_word []
-         else list_to_word (drop n (take word_width l)))`,
-   REPEAT GEN_TAC THEN
-   bool_cases_tac `LENGTH (l : bool list) <= word_width` THENL
-   [ASM_REWRITE_TAC [] THEN
-    MATCH_MP_TAC short_word_shr_list THEN
-    FIRST_ASSUM ACCEPT_TAC;
-    ASM_REWRITE_TAC [] THEN
-    MATCH_MP_TAC long_word_shr_list THEN
-    MATCH_MP_TAC LT_IMP_LE THEN
-    ASM_REWRITE_TAC [GSYM NOT_LE]]);;
-
-export_thm word_shr_list;;
-
-(*PARAMETRIC
-let word_shr_list = new_axiom
-   `!l n.
-      word_shr (list_to_word l) n =
-      (if LENGTH l <= word_width then
-         if LENGTH l <= n then list_to_word []
-         else list_to_word (drop n l)
-       else
-         if word_width <= n then list_to_word []
-         else list_to_word (drop n (take word_width l)))`;;
-*)
-
-let word_eq_bits = prove
-  (`!w1 w2. (!i. i < word_width ==> word_bit w1 i = word_bit w2 i) ==> w1 = w2`,
-   REPEAT GEN_TAC THEN
-   CONV_TAC (LAND_CONV (ONCE_REWRITE_CONV [GSYM word_to_list_to_word])) THEN
-   REWRITE_TAC [list_to_word_bit] THEN
-   STRIP_TAC THEN
-   MATCH_MP_TAC word_to_list_inj THEN
-   MATCH_MP_TAC nth_eq THEN
-   REWRITE_TAC [length_word_to_list] THEN
-   REPEAT STRIP_TAC THEN
-   FIRST_X_ASSUM (fun th -> MP_TAC (SPEC `i : num` th)) THEN
-   ASM_REWRITE_TAC [length_word_to_list]);;
-
-export_thm word_eq_bits;;
-
-(*PARAMETRIC
-let word_eq_bits = new_axiom
-  `!w1 w2. (!i. i < word_width ==> word_bit w1 i = word_bit w2 i) ==> w1 = w2`;;
-*)
-
-let num_to_word_cons = prove
-  (`!n.
-      list_to_word (CONS (ODD n) (word_to_list (num_to_word (n DIV 2)))) =
-      num_to_word n`,
-   GEN_TAC THEN
-   MATCH_MP_TAC word_to_num_inj THEN
-   REWRITE_TAC [cons_to_word_to_num] THEN
-   REWRITE_TAC [word_to_list_to_word] THEN
-   REWRITE_TAC [num_to_word_to_num] THEN
-   ONCE_REWRITE_TAC [GSYM mod_add_mod_word_size] THEN
-   ONCE_REWRITE_TAC [GSYM mod_mult_mod_word_size] THEN
-   REWRITE_TAC [mod_mod_refl_word_size] THEN
-   REWRITE_TAC [mod_mult_mod_word_size] THEN
-   REWRITE_TAC [mod_add_mod_word_size] THEN
-   AP_THM_TAC THEN
-   AP_TERM_TAC THEN
-   REWRITE_TAC [cond_mod_two] THEN
-   ONCE_REWRITE_TAC [MULT_SYM] THEN
-   MP_TAC (SPECL [`n : num`; `2`] DIVISION) THEN
-   COND_TAC THENL
-   [NUM_REDUCE_TAC;
-    ALL_TAC] THEN
-   DISCH_THEN (ACCEPT_TAC o SYM o CONJUNCT1));;
-
-export_thm num_to_word_cons;;
-
-(*PARAMETRIC
-let num_to_word_cons = new_axiom
-  `!n.
-     list_to_word (CONS (ODD n) (word_to_list (num_to_word (n DIV 2)))) =
-     num_to_word n`;;
-*)
-
-let num_to_word_list = prove
-  (`!n.
-      num_to_word n =
-      list_to_word
-        (if n = 0 then []
-         else CONS (ODD n) (word_to_list (num_to_word (n DIV 2))))`,
-   GEN_TAC THEN
-   bool_cases_tac `n = 0` THENL
-   [ASM_REWRITE_TAC [list_to_word_def];
-    ASM_REWRITE_TAC [num_to_word_cons]]);;
-
-export_thm num_to_word_list;;
-
-(*PARAMETRIC
-let num_to_word_list = new_axiom
-  `!n.
-     num_to_word n =
-     list_to_word
-       (if n = 0 then []
-        else CONS (ODD n) (word_to_list (num_to_word (n DIV 2))))`;;
-*)
-
-let word_lte_list = prove
-  (`!q w1 w2.
-      word_bits_lte q (word_to_list w1) (word_to_list w2) <=>
-      (if q then word_le w1 w2 else word_lt w1 w2)`,
-   REPEAT GEN_TAC THEN
-   MATCH_MP_TAC EQ_TRANS THEN
-   EXISTS_TAC `word_to_num w1 < word_to_num w2 + (if q then 1 else 0)` THEN
-   ONCE_REWRITE_TAC [CONJ_SYM] THEN
-   CONJ_TAC THENL
-   [BOOL_CASES_TAC `q : bool` THENL
-    [REWRITE_TAC [word_le_def; LT_SUC_LE; GSYM ADD1];
-     REWRITE_TAC [word_lt_def; ADD_0]];
-    ALL_TAC] THEN
-   CONV_TAC (RAND_CONV (ONCE_REWRITE_CONV [GSYM word_to_list_to_word])) THEN
-   KNOW_TAC
-     `LENGTH (word_to_list w1) <= word_width /\
-      LENGTH (word_to_list w2) <= word_width /\
-      LENGTH (word_to_list w1) = LENGTH (word_to_list w2)` THENL
-   [REWRITE_TAC [length_word_to_list; LE_REFL];
-    ALL_TAC] THEN
-   SPEC_TAC (`q : bool`,`q : bool`) THEN
-   SPEC_TAC (`word_to_list w2`,`l2 : bool list`) THEN
-   SPEC_TAC (`word_to_list w1`,`l1 : bool list`) THEN
-   LIST_INDUCT_TAC THENL
-   [LIST_INDUCT_TAC THENL
-    [GEN_TAC THEN
-     REWRITE_TAC [LT_ADD; word_bits_lte_def] THEN
-     BOOL_CASES_TAC `q : bool` THENL
-     [REWRITE_TAC [ONE; LT_0];
-      REWRITE_TAC [LT_REFL]];
-     REWRITE_TAC [LENGTH; NOT_SUC]];
-    ALL_TAC] THEN
-   LIST_INDUCT_TAC THENL
-   [REWRITE_TAC [LENGTH; NOT_SUC];
-    ALL_TAC] THEN
-   POP_ASSUM (K ALL_TAC) THEN
-   GEN_TAC THEN
-   REWRITE_TAC [cons_to_word_to_num; word_bits_lte_def; LENGTH; SUC_INJ] THEN
-   STRIP_TAC THEN
-   FIRST_X_ASSUM
-     (MP_TAC o SPECL [`t' : bool list`; `~h /\ h' \/ ~(h /\ ~h') /\ q`]) THEN
-   COND_TAC THENL
-   [ASM_REWRITE_TAC [] THEN
-    MATCH_MP_TAC LT_IMP_LE THEN
-    ASM_REWRITE_TAC [GSYM LE_SUC_LT];
-    ALL_TAC] THEN
-   DISCH_THEN (fun th -> REWRITE_TAC [th]) THEN
-   KNOW_TAC
-     `(2 * word_to_num (list_to_word t) + (if h then 1 else 0)) MOD word_size =
-      (2 * word_to_num (list_to_word t) + (if h then 1 else 0))` THENL
-   [MATCH_MP_TAC mod_lt_word_size THEN
-    MATCH_MP_TAC LTE_TRANS THEN
-    EXISTS_TAC `2 EXP SUC (LENGTH (t : bool list))` THEN
-    CONJ_TAC THENL
-    [MATCH_ACCEPT_TAC cons_to_word_to_num_bound;
-     REWRITE_TAC [word_size_def; le_exp_two] THEN
-     FIRST_ASSUM ACCEPT_TAC];
-    ALL_TAC] THEN
-   DISCH_THEN (fun th -> REWRITE_TAC [th]) THEN
-   KNOW_TAC
-     `(2 * word_to_num (list_to_word t') + (if h' then 1 else 0)) MOD word_size =
-      (2 * word_to_num (list_to_word t') + (if h' then 1 else 0))` THENL
-   [MATCH_MP_TAC mod_lt_word_size THEN
-    MATCH_MP_TAC LTE_TRANS THEN
-    EXISTS_TAC `2 EXP SUC (LENGTH (t' : bool list))` THEN
-    CONJ_TAC THENL
-    [MATCH_ACCEPT_TAC cons_to_word_to_num_bound;
-     REWRITE_TAC [word_size_def; le_exp_two] THEN
-     FIRST_ASSUM ACCEPT_TAC];
-    ALL_TAC] THEN
-   DISCH_THEN (fun th -> REWRITE_TAC [th]) THEN
-   POP_ASSUM_LIST (K ALL_TAC) THEN
-   SPEC_TAC (`word_to_num (list_to_word t)`, `m : num`) THEN
-   SPEC_TAC (`word_to_num (list_to_word t')`, `n : num`) THEN
-   REPEAT GEN_TAC THEN
-   BOOL_CASES_TAC `h : bool` THEN
-   BOOL_CASES_TAC `h' : bool` THEN
-   BOOL_CASES_TAC `q : bool` THEN
-   REWRITE_TAC [ADD_0; LT_ADD_RCANCEL; LT_MULT_LCANCEL] THEN
-   NUM_REDUCE_TAC THEN
-   ONCE_REWRITE_TAC [GSYM ADD1] THEN
-   REWRITE_TAC [LT_SUC_LE; LE_MULT_LCANCEL] THEN
-   NUM_REDUCE_TAC THENL
-   [REWRITE_TAC [GSYM LE_SUC_LT] THEN
-    REWRITE_TAC [ADD1] THEN
-    MATCH_MP_TAC EQ_TRANS THEN
-    EXISTS_TAC `2 * (m + 1) <= 2 * n` THEN
-    CONJ_TAC THENL
-    [REWRITE_TAC [LE_MULT_LCANCEL] THEN
-     NUM_REDUCE_TAC;
-     AP_THM_TAC THEN
-     AP_TERM_TAC THEN
-     REWRITE_TAC [LEFT_ADD_DISTRIB; GSYM ADD_ASSOC] THEN
-     NUM_REDUCE_TAC];
-    EQ_TAC THENL
-    [STRIP_TAC THEN
-     MATCH_MP_TAC LE_TRANS THEN
-     EXISTS_TAC `2 * n` THEN
-     ASM_REWRITE_TAC [LE_MULT_LCANCEL] THEN
-     ONCE_REWRITE_TAC [ADD_SYM] THEN
-     MATCH_ACCEPT_TAC LE_ADDR;
-     REWRITE_TAC [GSYM NOT_LT; CONTRAPOS_THM] THEN
-     REWRITE_TAC [GSYM LE_SUC_LT; ADD1] THEN
-     STRIP_TAC THEN
-     MATCH_MP_TAC LE_TRANS THEN
-     EXISTS_TAC `2 * (n + 1)` THEN
-     ASM_REWRITE_TAC [LE_MULT_LCANCEL] THEN
-     MATCH_MP_TAC EQ_IMP_LE THEN
-     REWRITE_TAC [LEFT_ADD_DISTRIB; GSYM ADD_ASSOC] THEN
-     NUM_REDUCE_TAC]]);;
-
-export_thm word_lte_list;;
-
-(*PARAMETRIC
-let word_lte_list = new_axiom
-   `!q w1 w2.
-      word_bits_lte q (word_to_list w1) (word_to_list w2) <=>
-      (if q then word_le w1 w2 else word_lt w1 w2)`;;
-*)
-
-let word_le_list = prove
-  (`!w1 w2.
-      word_bits_lte T (word_to_list w1) (word_to_list w2) <=> word_le w1 w2`,
-   REPEAT GEN_TAC THEN
-   MP_TAC (SPECL [`T`; `w1 : word`; `w2 : word`] word_lte_list) THEN
-   REWRITE_TAC []);;
-
-export_thm word_le_list;;
-
-(*PARAMETRIC
-let word_le_list = new_axiom
-   `!w1 w2.
-      word_bits_lte T (word_to_list w1) (word_to_list w2) <=> word_le w1 w2`;;
-*)
-
-let word_lt_list = prove
-  (`!w1 w2.
-      word_bits_lte F (word_to_list w1) (word_to_list w2) <=> word_lt w1 w2`,
-   REPEAT GEN_TAC THEN
-   MP_TAC (SPECL [`F`; `w1 : word`; `w2 : word`] word_lte_list) THEN
-   REWRITE_TAC []);;
-
-export_thm word_lt_list;;
-
-(*PARAMETRIC
-let word_lt_list = new_axiom
-   `!w1 w2.
-      word_bits_lte F (word_to_list w1) (word_to_list w2) <=> word_lt w1 w2`;;
-*)
-
-(* Word tactics *)
-
-(*PARAMETRIC
-let word_reduce_conv =
-    REWRITE_CONV
-      [word_to_num_to_word;
-       word_le_def; word_lt_def] THENC
-    REWRITE_CONV
-      [num_to_word_to_num] THENC
-    REWRITE_CONV
-      [word_width_def; word_size_def; num_to_word_eq] THENC
-    NUM_REDUCE_CONV;;
-*)
-
-(*PARAMETRIC
-let word_width_conv = REWR_CONV word_width_def;;
-
-let list_to_word_to_list_conv =
-    REWR_CONV list_to_word_to_list_eq THENC
-    cond_conv
-      (LAND_CONV length_conv THENC
-       RAND_CONV word_width_conv THENC
-       NUM_REDUCE_CONV)
-      (RAND_CONV
-         (RAND_CONV
-            (LAND_CONV word_width_conv THENC
-             RAND_CONV length_conv THENC
-             NUM_REDUCE_CONV) THENC
-          replicate_conv) THENC
-       append_conv)
-      (LAND_CONV word_width_conv THENC
-       take_conv);;
-
-let numeral_to_word_list_conv =
-    let zero_conv = REWR_CONV (SYM (CONJUNCT1 list_to_word_def)) in
-    let numeral_conv = REWR_CONV (SYM (SPEC `NUMERAL n` num_to_word_cons)) in
-    let rec rewr_conv tm =
-        (zero_conv ORELSEC
-         (numeral_conv THENC
-          RAND_CONV
-            (LAND_CONV NUM_REDUCE_CONV THENC
-             RAND_CONV
-               (RAND_CONV
-                  (RAND_CONV NUM_REDUCE_CONV THENC
-                   rewr_conv) THENC
-                list_to_word_to_list_conv)))) tm in
-    rewr_conv;;
-
-let word_and_list_conv =
-    let th = SPECL [`list_to_word l1`; `list_to_word l2`] word_and_def in
-    REWR_CONV th THENC
-    RAND_CONV
-      (LAND_CONV list_to_word_to_list_conv THENC
-       RAND_CONV list_to_word_to_list_conv THENC
-       zipwith_conv and_simp_conv);;
-
-let word_or_list_conv =
-    let th = SPECL [`list_to_word l1`; `list_to_word l2`] word_or_def in
-    REWR_CONV th THENC
-    RAND_CONV
-      (LAND_CONV list_to_word_to_list_conv THENC
-       RAND_CONV list_to_word_to_list_conv THENC
-       zipwith_conv or_simp_conv);;
-
-let word_shr_list_conv =
-    let th = SPECL [`l : bool list`; `NUMERAL n`] word_shr_list in
-    REWR_CONV th THENC
-    cond_conv
-      (RATOR_CONV (RAND_CONV length_conv) THENC
-       RAND_CONV word_width_conv THENC
-       NUM_REDUCE_CONV)
-      (cond_conv
-        (RATOR_CONV (RAND_CONV length_conv) THENC
-         NUM_REDUCE_CONV)
-        ALL_CONV
-        (RAND_CONV drop_conv))
-      (cond_conv
-        (RATOR_CONV (RAND_CONV word_width_conv) THENC
-         NUM_REDUCE_CONV)
-        ALL_CONV
-        (RAND_CONV
-           (RAND_CONV
-              (RATOR_CONV (RAND_CONV word_width_conv) THENC
-               take_conv) THENC
-            drop_conv)));;
-
-let word_shl_list_conv =
-    let th = SPECL [`l : bool list`; `NUMERAL n`] word_shl_list in
-    REWR_CONV th THENC
-    RAND_CONV
-      (LAND_CONV replicate_conv THENC
-       append_conv);;
-
-let word_bit_list_conv =
-    let th = SPECL [`l : bool list`; `NUMERAL n`] list_to_word_bit in
-    REWR_CONV th THENC
-    andalso_conv
-      (RAND_CONV word_width_conv THENC
-       NUM_REDUCE_CONV)
-      (andalso_conv
-        (RAND_CONV length_conv THENC
-         NUM_REDUCE_CONV)
-        nth_conv);;
-
-let word_bits_lte_conv =
-    let nil_conv = REWR_CONV (CONJUNCT1 word_bits_lte_def) in
-    let cons_conv = REWR_CONV (CONJUNCT2 word_bits_lte_def) in
-    let rec rewr_conv tm =
-        (nil_conv ORELSEC
-         (cons_conv THENC
-          (RATOR_CONV o RATOR_CONV o RAND_CONV)
-            ((RATOR_CONV o RAND_CONV)
-               (RATOR_CONV (RAND_CONV (TRY_CONV not_simp_conv)) THENC
-                TRY_CONV and_simp_conv) THENC
-             RAND_CONV
-               ((RATOR_CONV o RAND_CONV)
-                  (RAND_CONV
-                    (RAND_CONV (TRY_CONV not_simp_conv) THENC
-                     TRY_CONV and_simp_conv) THENC
-                   TRY_CONV not_simp_conv) THENC
-                TRY_CONV and_simp_conv) THENC
-             TRY_CONV or_simp_conv) THENC
-          rewr_conv)) tm in
-    rewr_conv;;
-
-let word_le_list_conv =
-    let th = SYM (SPECL [`list_to_word l1`; `list_to_word l2`] word_le_list) in
-    REWR_CONV th THENC
-    LAND_CONV list_to_word_to_list_conv THENC
-    RAND_CONV list_to_word_to_list_conv THENC
-    word_bits_lte_conv;;
-
-let word_lt_list_conv =
-    let th = SYM (SPECL [`list_to_word l1`; `list_to_word l2`] word_lt_list) in
-    REWR_CONV th THENC
-    LAND_CONV list_to_word_to_list_conv THENC
-    RAND_CONV list_to_word_to_list_conv THENC
-    word_bits_lte_conv;;
-
-let word_eq_list_conv =
-    let th = SYM (SPECL [`list_to_word l1`; `list_to_word l2`]
-                    word_to_list_inj_eq) in
-    REWR_CONV th THENC
-    LAND_CONV list_to_word_to_list_conv THENC
-    RAND_CONV list_to_word_to_list_conv THENC
-    list_eq_conv iff_simp_conv;;
-
-let word_bit_conv =
-    word_width_conv ORELSEC
-    list_to_word_to_list_conv ORELSEC
-    numeral_to_word_list_conv ORELSEC
-    word_and_list_conv ORELSEC
-    word_or_list_conv ORELSEC
-    word_shr_list_conv ORELSEC
-    word_shl_list_conv ORELSEC
-    word_bit_list_conv ORELSEC
-    word_le_list_conv ORELSEC
-    word_lt_list_conv ORELSEC
-    word_eq_list_conv;;
-
-let bit_blast_subterm_conv = word_bit_conv ORELSEC bit_blast_subterm_conv;;
-let bit_blast_conv = DEPTH_CONV bit_blast_subterm_conv;;
-let bit_blast_tac = CONV_TAC bit_blast_conv;;
-
-let prove_word_list_cases n =
-    let interval =
-        let rec intv i n = if n = 0 then [] else i :: intv (i + 1) (n - 1) in
-        intv 0 in
-    let lemma1 =
-        let nunary = funpow n (fun t -> mk_comb (`SUC`,t)) `0` in
-        let goal = mk_eq (`LENGTH (word_to_list w)`,nunary) in
-        let tac =
-            REWRITE_TAC [length_word_to_list; word_width_def] THEN
-            NUM_REDUCE_TAC in
-        prove (goal,tac) in
-    let witnesses =
-        let addtl l = mk_comb (`TL : bool list -> bool list`, hd l) :: l in
-        let tls = rev (funpow (n - 1) addtl [`l : bool list`]) in
-        map (fun t -> mk_comb (`HD : bool list -> bool`, t)) tls in
-    let goal =
-        let is = interval n in
-        let xs = map (fun i -> mk_var ("x" ^ string_of_int i, bool_ty)) is in
-        let w = mk_var ("w", `:word`) in
-        let body = mk_eq (w, mk_comb (`list_to_word`, mk_list (xs,bool_ty))) in
-        mk_forall (w, list_mk_exists (xs,body)) in
-    let tac =
-        GEN_TAC THEN
-        CONV_TAC
-          (funpow n (RAND_CONV o ABS_CONV)
-             (LAND_CONV (ONCE_REWRITE_CONV [GSYM word_to_list_to_word]))) THEN
-        MP_TAC lemma1 THEN
-        SPEC_TAC (`word_to_list w`, `l : bool list`) THEN
-        REPEAT STRIP_TAC THEN
-        EVERY (map EXISTS_TAC witnesses) THEN
-        AP_TERM_TAC THEN
-        POP_ASSUM MP_TAC THEN
-        N_TAC n
-          (MP_TAC (ISPEC `l : bool list` list_cases) THEN
-           STRIP_TAC THENL
-           [ASM_REWRITE_TAC [LENGTH; NOT_SUC];
-            ALL_TAC] THEN
-           POP_ASSUM SUBST_VAR_TAC THEN
-           REWRITE_TAC [LENGTH; SUC_INJ; HD; TL; CONS_11] THEN
-           SPEC_TAC (`t : bool list`, `l : bool list`) THEN
-           GEN_TAC) THEN
-        REWRITE_TAC [LENGTH_EQ_NIL] in
-    prove (goal,tac);;
-*)
+export_thm bits_to_num_to_bits;;
 
 logfile_end ();;
